theories/SpecNotations.v
@@ -14,6 +14,9 @@ Notation "'η'" := (eta) (at level 0).
 Notation "G ⊢ v ⇐ t" := (Jv G v t) (at level 90).
 Notation "G ⊢ V ⇒ t" := (JV G V t) (at level 90).
 
+Notation "ρ ⊢ v ⇓ v'" := (bigv ρ v v') (at level 90).
+(* Notation "ρ ⊢ V ⇓ v'" := (bigv ρ V v') (at level 90). *)
+
 Infix "|-" := P_with (at level 30).
 
 Module RelNotations.
